formal proofs

Program-proofs/Exercises/2D-counting/prob08/sol08PCStyle.dfy
@@ -1,24 +1,19 @@
-/* file: sol08.dfy
-   author: David De Potter
-   description: extra practice in Dafny, 2D counting, 
-   solution to prob08
-   This is exercise 9.9 from the PC reader
+/*  file: sol08PCStyle.dfy
+    author: David De Potter
+    description: extra practice in Dafny, 2D counting, 
+    solution to prob08
+    This is exercise 9.9 from the PC reader
+    NOTE: This solution follows the PC-style proof method described
+    in the general note on proof styles (see the README in the 
+    Exercises folder)
 */
 
-
-ghost predicate AscAsc(f:(int,int) -> int) 
-{
-  (forall i,j,k:: i <= j  ==>  f(i,k) <= f(j,k)) &&
-  (forall i,j,k:: j <= k  ==>  f(i,j) <= f(i,k))
-}
-
-function ord(b:bool): int
-{
-  if b then 1 else 0
-}
+include "../../commonSupport.dfy"
+import opened CommonFunctions
+import opened MonotonicityProps
 
 ghost function F(h:(int,int) -> int, x:nat, y:nat, n:nat): int
-requires AscAsc(h)
+requires Ordered2DInt(h, Asc, Asc)
 decreases x + (n - y)
 {
   if x == 0 || y >= n then 0
@@ -29,7 +24,7 @@ decreases x + (n - y)
 
 method problem08(h:(int,int) -> int, m:nat, n:nat) 
 returns (z: int)
-requires AscAsc(h)
+requires Ordered2DInt(h, Asc, Asc)
 ensures z == F(h,m,0,n)
 {
   var x:nat, y:nat := m, 0;
